\chapter{Esercizi} %Esercizi
\section{Esercizio 1 del 10/2/1989} %Esercizio 1 del 10/2/1989

\subsection{Risoluzione} %Risoluzione

%MANCA TUTTO

%MANCA UNA PARTE

Nella rappresentazione spettrale si ha:
\begin{equation}\begin{split}
U\left(t\right)=\\
=\exp{\left(-\frac{i}{\hbar }Ht\right)}=\\
=\exp{\left(-\frac{i}{\hbar }E_1t\right)}\left |E_1 \right\rangle\left\langle E_1\right |+\exp{\left(-\frac{i}{\hbar }E_2t\right)}\left |E_2 \right\rangle\left\langle E_2\right |
\end{split}\end{equation}

\begin{equation}\begin{split}
\left |\psi \left(t\right) \right\rangle=\begin{cases}
\left |\psi _1\left(t\right) \right\rangle=U\left(t\right)\left |E_1 \right\rangle, \textrm{     } p_1=\frac{1}{2}, & \left |\psi _1\left(t\right) \right\rangle=\exp{\left(-\frac{i}{\hbar }E_1t\right)}\left |E_1 \right\rangle\\
\left |\psi _2\left(t\right) \right\rangle=U\left(t\right)\left |E_2 \right\rangle, \textrm{     } p_2=\frac{1}{2}, & \left |\psi _2\left(t\right) \right\rangle=\exp{\left(-\frac{i}{\hbar }E_2t\right)}\left |E_2 \right\rangle
\end{cases}
\end{split}\end{equation}

%MANCA UNA PARTE

Mello stato miscela si ha:
\begin{equation}\begin{split}
\left |\psi \left(0\right) \right\rangle=\begin{cases}
\left |E_1 \right\rangle & p_1=\frac{1}{2}\\
\left |E_2 \right\rangle & p_2=\frac{1}{2}
\end{cases}
\end{split}\end{equation}

%MANCA TUTTO

In generale si ha:
\begin{equation}\begin{split}
\left |\psi \left(t\right) \right\rangle=\begin{cases}
\left |\psi _1\left(0\right) \right\rangle & p\ge 0 \\
\dots\\
\left |\psi _n\left(0\right) \right\rangle & p\ge 0
\end{cases}
\end{split}\end{equation}
\begin{equation}\begin{split}
\sum_i{p_i}=1\\
P\left(A=a_n\right)=\sum_{i=1}^{\infty }{p_i\left|\left\langle u_n|\psi _i\left(0\right) \right\rangle\right|^2}\\
\left\langle \hat A \right\rangle=
\end{split}\end{equation}

\begin{equation}\begin{split}
\sum_n{a_nP\left(A=a_n\right)}=\\
=\sum_n\sum_i{a_nP_i|\left\langle u_n|\psi _i \right\rangle|^2}\\
=\sum_i{p_i}\sum_n{\left\langle \psi _i|A|u_n \right\rangle\left\langle u_n|\psi _i \right\rangle}=\\
=\sum_i{p_i\left\langle \psi _i|A\left(\sum_n{\left |u_n \right\rangle\left\langle u_n\right |}\right)|\psi _i \right\rangle}=\\
=\sum_i{p_i\left\langle A \right\rangle_i}
\end{split}\end{equation}